src/LibListZ.v
@@ -13,182 +13,411 @@ Require Export LibContainer.
 
 Local Open Scope comp_scope.
 
+Ltac auto_tilde ::= eauto with maths.
+
 
 (* ********************************************************************** *)
 (** * List operations using indices in Z *)
 
-Section Zindices.
+(* ---------------------------------------------------------------------- *)
+(** * Length, with result as [int] *)
+
+(** Defined using a coercion from [nat] to [int] *)
+
+Definition length A (l:list A) : int :=
+  LibList.length l.
+
+Section Length.
 Variables A : Type.
 Implicit Types x : A.
 Implicit Types l : list A.
 Implicit Types i : int.
-Ltac auto_tilde ::= eauto with maths.
 
-
-(* ---------------------------------------------------------------------- *)
-(** * Definitions *)
-
-(** Functions *)
-
-Definition length (l:list A) :=
-  (length l) : int.
-
-Definition nth `{Inhab A} (i:int) (l:list A) :=
-  If i < 0 then arbitrary else nth (abs i) l.
-
-Definition update (i:int) (v:A) (l:list A) :=
-  If i < 0 then l else LibList.update (abs i) v l.
-
-Definition make (n:int) (v:A) :=
-  If n < 0 then arbitrary else make (abs n) v.
-
-End Zindices.
-
-
-(** Automation for [math], to unfold [length] *)
-
-Lemma LibListZ_length_def : forall A (l:list A),
+Lemma length_eq : forall l,
   length l = LibList.length l.
 Proof using. auto. Qed.
 
-Hint Rewrite LibListZ_length_def : rew_maths.
-
-(* DEMO: *)
-
-Goal forall A (l : list A), 0 <= length l.
-Proof using. intros. math. Qed.
-
-Goal forall (l : list Z) (s n : int),
-     s <= n -> s = length l -> n >= 0.
-Proof using. intros. math. Qed.
-
-
-(* ---------------------------------------------------------------------- *)
-(** ** Typeclasses read & update operations, binds and index predicates *)
-
-(** Note: we also define [card] as [length], but we use [length] everywhere
-    in the specifications. *)
-
-Definition card_impl A (l:list A) : nat :=
-  LibList.length l.
-  (* todo: should it return a nat or an int? might change... *)
-
-Definition read_impl `{Inhab A} (l:list A) (i:int) : A :=
-  nth i l.
-
-Definition update_impl A (l:list A) (i:int) (v:A) : list A :=
-  update i v l.
-
-Definition index_impl A (l:list A) (i:int) : Prop :=
-  index (LibList.length l : int) i.
-
-
-Instance card_inst : forall A, BagCard (list A).
- constructor. rapply (@card_impl A). Defined.
-Instance read_inst : forall `{Inhab A}, BagRead int A (list A).
- constructor. rapply (@read_impl A H). Defined.
-Instance update_inst : forall A, BagUpdate int A (list A).
-  constructor. rapply (@update_impl A). Defined.
-Instance index_inst : forall A, BagIndex int (list A).
-  constructor. rapply (@index_impl A). Defined.
-
-Global Opaque card_inst read_inst update_inst index_inst.
-
-(* LATER
-Definition binds_impl A (l:list A) (i:int) (v:A) : Prop :=
-  index_impl l i /\ nth i l = v.
-  (* deprecated:  ZNth i l v. *)
-Instance binds_inst : forall A, BagBinds int A (list A).
-  constructor. rapply (@binds_impl A). Defined.
-Global Opaque binds_inst
-*)
-
-(* ---------------------------------------------------------------------- *)
-(** * Properties of length *)
-
-Section LengthProperties.
-Variables (A : Type).
-Implicit Types l : list A.
-Ltac auto_tilde ::= eauto with maths.
-
-Lemma length_nonneg : forall (l: list A), 0 <= length l.
-Proof using. intros. math. Qed.
-Lemma length_nil :
-  length (@nil A) = 0.
-Proof using. auto. Qed.
-Lemma length_cons : forall x l,
-  length (x::l) = 1 + length l.
-Proof using. intros. unfold length. rew_length~. Qed.
-Lemma length_singleton: forall (x : A), length (x :: nil) = 1.
-Proof using. reflexivity. Qed.
-Lemma length_app : forall l1 l2,
-  length (l1 ++ l2) = length l1 + length l2.
-Proof using. intros. unfold length. rew_length~. Qed.
-Lemma length_last : forall x l,
-  length (l & x) = 1 + length l.
-Proof using. intros. unfold length. rew_length~. Qed.
-Lemma length_zero_inv : forall l,
-  length l = 0 -> l = nil.
-Proof using. intros. unfolds length. applys~ LibList.length_zero_inv. Qed.
-Lemma length_tail : forall l,
-  l <> nil -> length (tail l) = length l - 1.
-Proof using. induction l; intros; simpl; unfold length; rew_length. congruence. math. Qed.
-Lemma length_tail_le : forall l,
-  length (tail l) <= length l.
-Proof using. destruct l; simpl; unfold length; rew_length; math. Qed.
-Lemma length_le_1_implies_nil_tail : forall l,
-  length l <= 1 -> tail l = nil.
-Proof using.
-  intros. destruct l; eauto.
-  simpl. unfold length in *. rew_length in *.
-  eapply length_zero_inv. math.
-Qed.
-Lemma abs_length:
-  forall i l,
+Lemma abs_length : forall i l,
   i = length l ->
   abs i = LibList.length l.
-Proof using.
+Proof using. (* --TODO: cleanup proof *)
   unfold length. intros. subst.
   generalize (LibList.length l). clear A l. (* for clarity *)
   rew_maths. eapply Zabs2Nat.id.
 Qed.
 
-End LengthProperties.
+Lemma length_nonneg : forall (l: list A), 
+  0 <= length l.
+Proof using. intros. rewrite length_eq. math. Qed.
+
+Lemma length_nil :
+  length (@nil A) = 0.
+Proof using. auto. Qed.
+
+Lemma length_cons : forall x l,
+  length (x::l) = 1 + length l.
+Proof using. intros. unfold length. rew_list~. Qed.
+
+Lemma length_one: forall x,
+  length (x::nil) = 1.
+Proof using. reflexivity. Qed.
+
+Lemma length_app : forall l1 l2,
+  length (l1 ++ l2) = length l1 + length l2.
+Proof using. intros. unfold length. rew_list~. Qed.
+
+Lemma length_last : forall x l,
+  length (l & x) = 1 + length l.
+Proof using. intros. unfold length. rew_list~. Qed.
+
+Lemma length_zero_inv : forall l,
+  length l = 0 -> 
+  l = nil.
+Proof using. intros. unfolds length. applys~ LibList.length_zero_inv. Qed.
+
+(*-- TODO: there is no lemmas about [tail] in LibList;
+     should we keep these? *)
+(*
+Lemma length_tail : forall l,
+  l <> nil -> 
+  length (tail l) = length l - 1.
+Proof using. induction l; intros; simpl; unfold length; rew_list. congruence. math. Qed.
+
+Lemma length_tail_le : forall l,
+  length (tail l) <= length l.
+Proof using. destruct l; simpl; unfold length; rew_list; math. Qed.
+
+Lemma length_le_1_inv_tail_eq_nil : forall l,
+  length l <= 1 -> 
+  tail l = nil.
+Proof using.
+  intros. destruct l; eauto.
+  simpl. unfold length in *. rew_list in *.
+  eapply length_zero_inv. math.
+Qed.
+*)
+
+End Length.
 
 Hint Rewrite length_nil length_cons length_app
- length_last length_rev : rew_length.
-Hint Rewrite length_nil length_cons length_app
  length_last length_rev : rew_list.
+ (* --TODO: should we use a separate [rew_listZ] data base ? *)
+
+(** Automation for [math], to unfold [length] *)
+
+Hint Rewrite length_eq : rew_maths.
+
+(** Demo of automation with maths *)
+
+Goal forall A (l : list A), 0 <= length l.
+Proof using. intros. math. Qed.
+
+Goal forall (l : list Z) (s n : int), 
+  s <= n -> 
+  s = length l -> 
+  n >= 0.
+Proof using. intros. math. Qed.
 
 
 (* ---------------------------------------------------------------------- *)
-(** * Properties of zmake *)
+(** * [index], with length as [int], as typeclass *)
 
-Section MakeProperties.
-Transparent read_inst.
+Definition index_impl A (l:list A) (i:int) : Prop :=
+  index (LibList.length l : int) i.
 
-Lemma read_make : forall `{Inhab A} (i n:int) (v:A),
-  index n i -> (make n v)[i] = v.
+Instance index_inst : forall A, BagIndex int (list A).
+Proof using. constructor. rapply (@index_impl A). Defined.
+
+Section Index.
+Variables (A : Type).
+Implicit Types l : list A.
+Implicit Types n i : int.
+
+Lemma index_eq_inbound : forall l i,
+  index l i = (0 <= i < length l).
+Proof using. auto. Qed.
+
+Lemma index_of_inbound : forall l i,
+  0 <= i < length l -> 
+  index l i.
+Proof using. intros. rewrite~ index_eq_inbound. Qed.
+
+Lemma index_eq_index_length : forall l i,
+  index l i = index (length l) i.
+Proof using. auto. Qed.
+
+Lemma index_of_index_length : forall l i,
+  index (length l) i -> 
+  index l i.
+Proof using. introv H. rewrite* index_eq_index_length. Qed.
+
+(** Reformulation of above, helpful for automation *)
+
+Lemma index_of_index_length' : forall l n i,
+  index n i -> 
+  n = length l -> 
+  index l i.
+Proof using. intros. subst. rewrite~ index_eq_index_length. Qed.
+
+End Index.
+
+Global Opaque index_inst.
+
+
+(* ---------------------------------------------------------------------- *)
+(** * [read], with length as [int], as typeclass *)
+
+Definition read_impl `{Inhab A} (l:list A) (i:int) : A :=
+  If i < 0 then arbitrary else nth (abs i) l.
+
+Instance read_inst : forall `{Inhab A}, BagRead int A (list A).
+Proof using. constructor. rapply (@read_impl A H). Defined.
+
+Section Read.
+Context (A : Type) `{Inhab A}.
+Implicit Types x : A.
+Implicit Types l : list A.
+Implicit Types n i : int.
+
+Lemma read_cons_case : forall l i v,
+  (v::l)[i] = (If i = 0 then v else l[i-1]).
 Proof using.
-  introv N. rewrite int_index_eq in N. unfold make, read_inst, read_impl, nth.
-  case_if. math. simpl. case_if. math.
-  applys nth_make. forwards: lt_abs_abs i n; try math.
+  introv. simpl. unfold read_impl. case_if.
+  { case_if. math. case_if~. math. }
+  { case_if~.
+    { subst. rewrite abs_0. rew_listx~. }
+    { rewrite~ abs_eq_succ_abs_minus_one. rew_listx.
+      case_if. math. auto. } }
 Qed.
 
-Lemma length_make : forall A (n:int) (v:A),
+Lemma read_cons_zero : forall x l,
+  (x::l)[0] = x.
+Proof using. 
+  intros. rewrite read_cons_case. case_if. auto. 
+Qed.
+
+Lemma read_cons_succ : forall x l i,
+  0 <= i < length l ->
+  (x::l)[i+1] = l[i].
+Proof using.
+  introv M. rewrite read_cons_case. case_if. { math. }  
+  fequals. math.
+Qed.
+
+(*--TODO: unclear if next lemma should be using [length] of [LibList.length] *)
+
+Lemma read_last_case : forall l i v,
+  (l & v)[i] = (If i = LibList.length l then v else l[i]).
+Proof using.
+  introv. simpl. unfold read_impl. case_if.
+  { case_if~; math. } 
+  { rewrite nth_last. rewrite~ abs_eq_nat_eq. }
+Qed.
+
+End Read.
+
+Global Opaque read_inst.
+
+
+(* ---------------------------------------------------------------------- *)
+(** * Equality between two lists from equality of length and 
+      extensional equality of reads. *)
+
+Lemma eq_of_extensional : forall `{Inhab A} (l1 l2:list A),
+  length l1 = length l2 ->
+  (forall i, 0 <= i < length l1 -> l1[i] = l2[i]) ->
+  l1 = l2.
+Proof using. (* --LATER: cleanup proof *)
+  induction l1; destruct l2; simpl; introv Heq Hread;
+  try solve [ eauto | false ]. f_equal.
+  { specializes Hread 0.
+    repeat rewrite read_cons_zero in Hread.
+    repeat rewrite length_cons in Hread.
+    eapply Hread.
+    forwards: length_nonneg l1. math. }
+  { repeat rewrite length_cons in *.
+    eapply IHl1. math. intros i Hi.
+    specializes Hread (i + 1).
+    do 2 rewrite read_cons_succ in Hread by math.
+    eapply Hread. math. }
+Qed.
+
+Lemma eq_of_extensional_using_index : forall `{Inhab A} (l1 l2:list A),
+  length l1 = length l2 ->
+  (forall i, index l1 i -> l1[i] = l2[i]) ->
+  l1 = l2.
+Proof using. intros. applys~ eq_of_extensional. Qed.
+
+
+(* ---------------------------------------------------------------------- *)
+(** * [update], with index as [int], as typeclass *)
+
+Definition update_impl A (l:list A) (i:int) (v:A) : list A :=
+  If i < 0 then l else LibList.update (abs i) v l.
+
+Instance update_inst : forall A, BagUpdate int A (list A).
+Proof using. constructor. rapply (@update_impl A). Defined.
+
+Section Update.
+Transparent index_inst read_inst update_inst.
+Context (A : Type) `{IA:Inhab A}.
+Implicit Types x v w : A.
+Implicit Types l : list A.
+Implicit Types i j : int.
+
+Lemma length_update : forall l i v,
+  length (l[i:=v]) = length l.
+Proof using.
+  intros. unfold update_inst, update_impl, length, update. simpl.
+  case_if. math. rewrite~ length_update.
+Qed.
+
+Lemma index_update_eq : forall l i j v,
+  index (l[j:=v]) i = index l i.
+Proof using. intros. rewrite index_eq_index_length in *. rewrite~ length_update. Qed.
+
+Lemma index_update : forall l i j v,
+  index l i -> 
+  index (l[j:=v]) i.
+Proof using. intros. rewrite~ index_update_eq. Qed.
+
+Lemma read_update_case : forall l i j v,
+  index l j ->
+  l[i:=v][j] = (If i = j then v else l[j]).
+Proof using.
+  introv. unfold index_inst, index_impl, update_inst, update_impl, update,
+    read_inst, read_impl. simpl. introv N. rewrite int_index_eq in N.
+  case_if. math.
+  case_if. case_if. auto. case_if.
+    subst. rewrite~ nth_update_eq. apply lt_nat_of_lt_int. rewrite abs_pos; try math.
+    rewrite~ nth_update_neq. apply lt_nat_of_lt_int. rewrite abs_pos; try math.
+      apply neq_nat_of_neq_int. rewrite abs_pos; try math. rewrite abs_pos; try math.
+Qed.
+
+Lemma read_update_same : forall l i v,
+  index l i -> 
+  (l[i:=v])[i] = v.
+Proof using. introv N. rewrite~ read_update_case. case_if~. Qed.
+
+Lemma read_update_neq : forall l i j v,
+  index l j ->
+  (i <> j) -> 
+  (l[i:=v])[j] = l[j].
+Proof using. introv N. rewrite~ read_update_case. case_if; auto_false~. Qed.
+
+Lemma update_update_same : forall l i v w,
+  index l i ->
+  l[i:=v][i:=w] = l[i:=w].
+Proof using. (* --TODO: cleanup proof *)
+  intros. eapply ext_eq_index; repeat rewrite length_update.
+  { reflexivity. }
+  intros j.
+  repeat rewrite index_update_eq.
+  intros Hj.
+  repeat rewrite read_update_case by eauto using index_update.
+  case_if; reflexivity.
+Qed.
+
+Lemma update_update_neq : forall l i j v w,
+  index l i -> 
+  index l j -> 
+  i <> j -> 
+  l[i:=v][j:=w] = l[j:=w][i:=v].
+Proof using. (* --TODO: cleanup proof *)
+  intros. eapply ext_eq_index; repeat rewrite length_update.
+  { reflexivity. }
+  intros k.
+  repeat rewrite index_update_eq.
+  intros Hk.
+  repeat rewrite read_update_case by eauto using index_update.
+  repeat case_if; reflexivity.
+Qed.
+
+(*-- TODO: add lemma update_app_l *)
+
+Lemma update_app_r : forall l2 j l1 i ij v,
+  i = length l1 ->
+  0 <= j ->
+  ij = i + j ->
+  (l1 ++ l2)[ij:=v] = l1 ++ (l2[j:=v]).
+Proof using. (* --TODO: cleanup proof *)
+  intros. subst ij.
+  unfold LibContainer.update, update_inst, update_impl.
+  unfold update. do 2 (case_if; [ math | ]).
+  eapply LibList.update_app_right with (i := abs i).
+  { eauto using abs_length. }
+  { eapply Zabs2Nat.inj_add; math. }
+Qed.
+
+Lemma update_app_middle : forall i l1 l2 v w,
+  i = length l1 ->
+  (l1 ++ w :: l2)[i := v] = l1 & v ++ l2.
+Proof using. (* --TODO: cleanup proof *)
+  intros.
+  unfold LibContainer.update, update_inst, update_impl.
+  unfold update. case_if; [ math | ].
+  eapply LibList.update_app_right_here.
+  eauto using abs_length.
+Qed.
+
+End Update.
+
+Global Opaque update_inst.
+
+
+
+(* ---------------------------------------------------------------------- *)
+(** * [make], with length as [int] *)
+
+Definition make A (n:int) (v:A) : list A :=
+  If n < 0 then arbitrary else make (abs n) v.
+
+Section Make.
+Transparent index_inst read_inst.
+Variables A : Type.
+Implicit Types x v : A.
+Implicit Types l : list A.
+Implicit Types n i : int.
+
+Lemma index_make : forall n i v,
+  index n i ->
+  index (make n v) i.
+Proof using.
+  introv H. rewrite index_eq_index_length. rewrite int_index_eq in H.
+  rewrite~ length_make. math.
+Qed.
+
+Lemma length_make : forall n v,
   n >= 0 ->
-  length (make n v) = n :> int.
+  length (make n v) = n.
 Proof using.
   introv N. unfold make. case_if. math.
   unfold length. rewrite LibList.length_make.
   rewrite~ abs_pos.
 Qed.
 
-Lemma cons_make: forall n A (x : A), 0 < n -> x :: make (n - 1) x = make n x.
+Lemma read_make : forall i n v,
+  index n i -> 
+  (make n v)[i] = v.
 Proof using.
+  introv N. rewrite int_index_eq in N. 
+  unfold make, read_inst, read_impl, nth.
+  case_if. math. simpl. case_if. math.
+  applys nth_make. forwards: lt_abs_abs i n; try math.
+Qed.
+
+(*-- LATER:
+Lemma cons_make_same : forall n x, 
+  0 <= n -> 
+  x::(make n x) = make (n+1) x.
+*)
+
+Lemma cons_make_pred_same : forall n x, 
+  0 < n -> 
+  x::(make (n - 1) x) = make n x.
+Proof using. (* --TODO: cleanup proof *)
   intros.
   unfold make. do 2 (case_if; [ math | ]).
-  (* This is really painful. *)
   rewrite abs_minus by math.
   change (abs 1) with 1%nat.
   assert (0 < abs n)%nat.
@@ -199,222 +428,70 @@ Proof using.
   math.
 Qed.
 
-End MakeProperties.
+End Make.
 
-
-(* -------------------------------------------------------------------------- *)
-
-(* Properties of [read]. *)
-
-Section ReadProperties.
-Transparent read_inst.
-
-Context (A : Type) `{Inhab A}.
-
-Lemma read_zero:
-  forall x (xs : list A),
-  (x :: xs)[0] = x.
-Proof using.
-  intros. unfold read, read_inst, read_impl, nth.
-  case_if; [ math | ]. reflexivity.
-Qed.
-
-Lemma read_succ:
-  forall x (xs : list A) i,
-  0 <= i < length xs ->
-  (x :: xs)[i + 1] = xs[i].
-Proof using.
-  intros. unfold read, read_inst, read_impl, nth, LibList.nth.
-  do 2 (case_if; [ math | ]).
-  change (i + 1) with (Z.succ i).
-  rewrite Zabs2Nat.inj_succ by math.
-  reflexivity.
-Qed.
-
-End ReadProperties.
 
 (* ---------------------------------------------------------------------- *)
-(* Extensional equality between two lists. *)
+(** * [card], with result as [nat], as typeclass *)
 
-Lemma ext_eq:
-  forall A `{Inhab A} (xs ys : list A),
-  length xs = length ys ->
-  (forall i, 0 <= i < length xs -> xs[i] = ys[i]) ->
-  xs = ys.
-Proof using.
-  induction xs; destruct ys; simpl; introv Heq Hread;
-  try solve [ eauto | false ]. f_equal.
-  (* The head. *)
-  { specializes Hread 0.
-    repeat rewrite read_zero in Hread.
-    repeat rewrite length_cons in Hread.
-    eapply Hread.
-    forwards: length_nonneg xs. math. }
-  (* The tail. *)
-  { repeat rewrite length_cons in *.
-    eapply IHxs. math. intros i Hi.
-    specializes Hread (i + 1).
-    do 2 rewrite read_succ in Hread by math.
-    eapply Hread. math. }
-Qed.
+(** Note that [card] produces a [nat], whereas [length] produces an [int]. 
+    Currently, in practice, we use [LibList.length] rather than [card]. *)
 
-Lemma ext_eq_index:
-  forall A `{Inhab A} (xs ys : list A),
-  length xs = length ys ->
-  (forall i, index xs i -> xs[i] = ys[i]) ->
-  xs = ys.
-Proof using.
-  eauto using ext_eq.
-Qed.
+Definition card_impl A (l:list A) : nat :=
+  LibList.length l.
+
+Instance card_inst : forall A, BagCard (list A).
+Proof using. constructor. rapply (@card_impl A). Defined.
+
+Global Opaque card_inst.
+
 
 (* ---------------------------------------------------------------------- *)
-(** * Properties of update *)
+(** * [binds], with length as [int], as typeclass *)
 
-Section UpdateProperties.
-Transparent index_inst read_inst update_inst.
+(* --LATER: is this any useful?
 
-Lemma index_def : forall A (l:list A) i,
-  index l i = index (length l : int) i.
-Proof using. auto. Qed.
+  Definition binds_impl A (l:list A) (i:int) (v:A) : Prop :=
+    index_impl l i /\ nth i l = v.
 
-Lemma length_update : forall A (l:list A) (i:int) (v:A),
-  length (l[i:=v]) = length l.
-Proof using.
-  intros. unfold update_inst, update_impl, length, update. simpl.
-  case_if. math. rewrite~ length_update.
-Qed.
+  Instance binds_inst : forall A, BagBinds int A (list A).
+  Proof using. constructor. rapply (@binds_impl A). Defined.
 
-Lemma index_update_eq : forall A (l:list A) i j (v:A),
-  index (l[j:=v]) i = index l i.
-Proof using. intros. rewrite index_def in *. rewrite~ length_update. Qed.
+  Global Opaque binds_inst
 
-Lemma index_update : forall A (l:list A) i j (v:A),
-  index l i -> index (l[j:=v]) i.
-Proof using. intros. rewrite~ index_update_eq. Qed.
-
-Lemma read_update_case : forall `{Inhab A} (l:list A) (i j:int) (v:A),
-  index l j -> l[i:=v][j] = (If i = j then v else l[j]).
-Proof using.
-  introv. unfold index_inst, index_impl, update_inst, update_impl, update,
-    read_inst, read_impl, nth. simpl. introv N. rewrite int_index_eq in N.
-  case_if. math.
-  case_if. case_if. auto. case_if.
-    rewrite~ nth_update_eq. apply lt_nat_of_lt_int. rewrite abs_pos; try math.
-    rewrite~ nth_update_neq. apply lt_nat_of_lt_int. rewrite abs_pos; try math.
-      apply neq_nat_of_neq_int. rewrite abs_pos; try math. rewrite abs_pos; try math.
-Qed.
-
-Lemma read_update_eq : forall `{Inhab A} (l:list A) (i:int) (v:A),
-  index l i -> (l[i:=v])[i] = v.
-Proof using. introv N. rewrite~ read_update_case. case_if~. Qed.
-
-Lemma read_update_neq : forall `{Inhab A} (l:list A) (i j:int) (v:A),
-  index l j -> (i <> j) -> (l[i:=v])[j] = l[j].
-Proof using. introv N. rewrite~ read_update_case. case_if; auto_false~. Qed.
-
-Lemma update_update_eq : forall `{Inhab A} (l:list A) (i:int) (v w:A),
-  index l i -> l[i:=v][i:=w] = l[i:=w].
-Proof using.
-  intros. eapply ext_eq_index; repeat rewrite length_update.
-  { reflexivity. }
-  intros j.
-  repeat rewrite index_update_eq.
-  intros Hj.
-  repeat rewrite read_update_case by eauto using index_update.
-  case_if; reflexivity.
-Qed.
-
-Lemma update_update_neq : forall `{Inhab A} (l:list A) (i j:int) (v w:A),
-  index l i -> index l j -> i <> j -> l[i:=v][j:=w] = l[j:=w][i:=v].
-Proof using.
-  intros. eapply ext_eq_index; repeat rewrite length_update.
-  { reflexivity. }
-  intros k.
-  repeat rewrite index_update_eq.
-  intros Hk.
-  repeat rewrite read_update_case by eauto using index_update.
-  repeat case_if; reflexivity.
-Qed.
-
-Lemma update_app_right:
-  forall A ys j xs i ij (v : A),
-  i = length xs ->
-  0 <= j ->
-  ij = i + j ->
-  (xs ++ ys)[ij:=v] = xs ++ ys[j:=v].
-Proof using.
-  intros. subst ij.
-  unfold LibContainer.update, update_inst, update_impl.
-  unfold update. do 2 (case_if; [ math | ]).
-  eapply LibList.update_app_right with (i := abs i).
-  { eauto using abs_length. }
-  { eapply Zabs2Nat.inj_add; math. }
-Qed.
-
-Lemma update_app_right_here:
-  forall A i (xs ys : list A) x y,
-  i = length xs ->
-  (xs ++ y :: ys)[i := x] = xs & x ++ ys.
-Proof using.
-  intros.
-  unfold LibContainer.update, update_inst, update_impl.
-  unfold update. case_if; [ math | ].
-  eapply LibList.update_app_right_here.
-  eauto using abs_length.
-Qed.
-
-Lemma read_cons_case : forall `{IA:Inhab A} (l:list A) (i:int) (v:A),
-  (v::l)[i] = (If i = 0 then v else l[i-1]).
-Proof using.
-  introv. simpl. unfold read_impl, nth.
-  case_if.
-  - case_if. math. case_if~. math.
-  - case_if~. case_if. math. rewrite~ abs_to_succ_abs_minus_one. math.
-Qed.
-
-Lemma read_last_case : forall `{IA:Inhab A} (l:list A) (i:int) (v:A),
-  (l & v)[i] = (If i = LibList.length l then v else l[i]).
-Proof using.
-  introv. simpl. unfold read_impl, nth.
-  case_if.
-  - case_if~; math.
-  - admit. (* lemmas missing about "&" and LibList.nth *)
-Qed.
-
-End UpdateProperties.
+*)
 
 
 (* ---------------------------------------------------------------------- *)
 (** * Normalization tactics *)
 
-(** [rew_arr] is a light normalization tactic for array *)
+(** [rew_array_nocase] is a light normalization tactic for array *)
 
-(* TODO: rename to [rew_array_nocase] *)
 Hint Rewrite @read_make @length_make @length_update @read_update_eq
-  : rew_arr.
+  : rew_array_nocase.
 
-Tactic Notation "rew_arr" :=
-  autorewrite with rew_arr.
+Tactic Notation "rew_array_nocase" :=
+  autorewrite with rew_array_nocase.
 Tactic Notation "rew_arr" "in" hyp(H) :=
-  autorewrite with rew_arr in H.
+  autorewrite with rew_array_nocase in H.
 Tactic Notation "rew_arr" "in" "*" :=
-  autorewrite_in_star_patch ltac:(fun tt => autorewrite with rew_arr).
-  (* autorewrite with rew_arr in *. *)
-
+  autorewrite_in_star_patch ltac:(fun tt => autorewrite with rew_array_nocase).
+  (* autorewrite with rew_array_nocase in *. *)
 Tactic Notation "rew_arr" "~" :=
-  rew_arr; auto_tilde.
+  rew_array_nocase; auto_tilde.
 Tactic Notation "rew_arr" "*" :=
-  rew_arr; auto_star.
+  rew_array_nocase; auto_star.
 Tactic Notation "rew_arr" "~" "in" hyp(H) :=
-  rew_arr in H; auto_tilde.
+  rew_array_nocase in H; auto_tilde.
 Tactic Notation "rew_arr" "*" "in" hyp(H) :=
-  rew_arr in H; auto_star.
+  rew_array_nocase in H; auto_star.
 Tactic Notation "rew_arr" "~" "in" "*" :=
-  rew_arr in *; auto_tilde.
+  rew_array_nocase in *; auto_tilde.
 Tactic Notation "rew_arr" "*" "in" "*" :=
-  rew_arr in *; auto_star.
+  rew_array_nocase in *; auto_star.
 
-(** [rew_array] is a normalization tactic for array *)
+(** [rew_array] is a normalization tactic for array, which introduces
+    case analyses for all read-on-update operations. *)
 
 Hint Rewrite @read_make @length_make @length_update @read_update_eq
   @read_update_case @read_cons_case @read_last_case : rew_array.
@@ -426,7 +503,6 @@ Tactic Notation "rew_array" "in" hyp(H) :=
 Tactic Notation "rew_array" "in" "*" :=
   autorewrite_in_star_patch ltac:(fun tt => autorewrite with rew_array).
   (* autorewrite with rew_array in *. *)
-
 Tactic Notation "rew_array" "~" :=
   rew_array; auto_tilde.
 Tactic Notation "rew_array" "*" :=
@@ -440,372 +516,9 @@ Tactic Notation "rew_array" "~" "in" "*" :=
 Tactic Notation "rew_array" "*" "in" "*" :=
   rew_array in *; auto_star.
 
-(* ---------------------------------------------------------------------- *)
-(** * Valid index predicate *)
-
-Section IndexProperties.
-Transparent index_inst.
-
-(* [index_def] : proven above *)
-
-(* [index_update] : proven above *)
-
-Lemma index_length_unfold : forall A (l:list A) i,
-  index (length l : int) i -> index l i.
-Proof using. introv H. rewrite* index_def. Qed.
-
-Lemma index_length_eq : forall A (l:list A) (n:int) i,
-  index n i -> n = length l -> index l i.
-Proof using. intros. subst. rewrite~ index_def. Qed.
-
-Lemma index_bounds : forall A (l:list A) i,
-  index l i = (0 <= i < length l).
-Proof using. auto. Qed.
-
-Lemma index_bounds_impl : forall A (l:list A) i,
-  0 <= i < length l -> index l i.
-Proof using. intros. rewrite~ index_bounds. Qed.
-
-Lemma index_zmake : forall A n i (v:A),
-  index n i -> index (make n v) i.
-Proof using.
-  introv H. rewrite index_def. rewrite int_index_eq in H.
-  rewrite~ length_make. math.
-Qed.
-
-End IndexProperties.
-
-
-(* ---------------------------------------------------------------------- *)
-(** * count *)
-
-(* UNDER CONSTRUCTION *)
-
-(* TODO: complete definitions and proofs, which are used by CFML/Dijstra *)
-
-Require Import LibWf.
-
-(* TODO: implement a non-decidable version of count *)
-
-Axiom count : (* UNDER CONSTRUCTION *)
-  forall A (P:A->Prop) (l:list A), int.
-
-(* currently not used
-  Axiom count_make : forall A (f:A->Prop) n v,
-    count f (make n v) = (If f v then n else 0).
-*)
-
-Axiom count_update : (* UNDER CONSTRUCTION *)
-  forall `{Inhab A} (P:A->Prop) (l:list A) (i:int) v,
-  index l i ->
-  count P (l[i:=v]) = count P l
-    - (If P (l[i]) then 1 else 0)
-    + (If P v then 1 else 0).
-
-Axiom count_bounds : (* UNDER CONSTRUCTION *)
-  forall `{Inhab A} (l:list A) (P:A->Prop),
-  0 <= count P l <= length l.
-
-(** The following lemma is used to argue that the update to a sequence,
-    when writing a value that satisfies [P] in place of one that did not
-    satisfy [P], decreases the total number of values that satisfying
-    [P] in the sequence. *)
-
-Lemma count_upto : forall `{Inhab A} (P:A->Prop) (l:list A) (n i:int) (v:A),
-  ~ P (l[i]) -> P v -> index l i -> (length l <= n)%Z ->
-  upto n (count P (l[i:=v])) (count P l).
-Proof using.
-  introv Ni Pv Hi Le. forwards K: (count_bounds (l[i:=v]) P). split.
-  rewrite length_update in K. math.
-  lets M: (@count_update A _). rewrite~ M. clear M.
-  do 2 (case_if; tryfalse). math.
-Qed.
-
-
-
-(* ---------------------------------------------------------------------- *)
-(* LATER:
-
-Lemma isTrue_eq_list : forall A {IA:Inhab A} (L1 L2:list A),
-  len L1 = len L2 ->
-  ((forall i, index (len L1) i -> L1[i] = L2[i]) ->
-  (L1 = L2)).
-
-*)
-
-
-
 
 
 (* ********************************************************************** *)
-(** * DEPRECATED -- List predicates using indices in Z *)
+(** Restore automation *)
 
-Section ZindicesOld.
-Variables A : Type.
-Implicit Types x : A.
-Implicit Types l : list A.
-Implicit Types i : int.
-Ltac auto_tilde ::= eauto with maths.
-
-(* ---------------------------------------------------------------------- *)
-(** * DEPRECATED *)
-
-(** Predicates *)
-
-Definition ZInbound i l :=
-  0 <= i /\ i < length l.
-
-Definition ZNth i l x :=
-  Nth (abs i) l x /\ 0 <= i.
-
-Definition ZUpdate i x l l' :=
-  Update (abs i) x l l' /\ 0 <= i.
-
-
-(* ---------------------------------------------------------------------- *)
-(** * DEPRECATED -- Znth *)
-
-Lemma ZNth_here : forall i x l,
-  i = 0 -> ZNth i (x::l) x.
-Proof using. intros. subst. split~. constructor. Qed.
-
-Lemma ZNth_zero : forall x l,
-  ZNth 0 (x::l) x.
-Proof using. intros. apply~ ZNth_here. Qed.
-
-Lemma ZNth_next : forall i j x y l,
-  ZNth j l x -> i = j+1 -> ZNth i (y::l) x.
-Proof using.
-  introv [H P] M. subst. split~.
-  applys_eq* Nth_next 3. rew_abs_pos~.
-Qed.
-
-Lemma ZNth_app_l : forall i x l1 l2,
-  ZNth i l1 x -> ZNth i (l1 ++ l2) x.
-Proof using. introv [H P]. split~. apply~ Nth_app_l. Qed.
-
-Lemma ZNth_app_r : forall i j x l1 l2,
-  ZNth j l2 x -> i = j + length l1 -> ZNth i (l1 ++ l2) x.
-Proof using.
-  introv [H P]. unfold length. split~. subst.
-  apply* Nth_app_r. rew_abs_pos~.
-Qed.
-
-Lemma ZNth_nil_inv : forall i x,
-  ZNth i nil x -> False.
-Proof using. introv [H P]. apply* Nth_nil_inv. Qed.
-
-Lemma ZNth_cons_inv : forall i x l,
-  ZNth i l x ->
-     (exists q, l = x::q /\ i = 0)
-  \/ (exists y q j, l = y::q /\ ZNth j q x /\ i = j+1).
-Proof using.
-  introv [H P]. forwards~: (@abs_pos i).
-  destruct (Nth_cons_inv H); unpack.
-  left. exists___. split~.
-  right. exists___. splits~.
-   split. rewrite* abs_pos_nat. math.
-   math.
-Qed.
-
-Lemma ZNth_inbound : forall i l,
-   ZInbound i l -> exists x, ZNth i l x.
-Proof using.
-  introv [P U]. unfolds length. gen_eq n: (abs i).
-  gen i l. induction n; intros;
-    forwards~: (@abs_pos i); destruct l; rew_length in U; try math.
-  math_rewrite (i = 0). exists __. split~. constructor.
-  forwards~ [x [M P']]: (>> IHn (i-1) l).
-    forwards~: (@abs_to_succ_abs_minus_one i).
-    exists x. split~. rewrite~ (@abs_to_succ_abs_minus_one i). constructor~.
-Qed.
-
-
-(* ---------------------------------------------------------------------- *)
-(** * DEPRECATED -- ZInbound *)
-
-Lemma ZInbound_zero : forall x l,
-  ZInbound 0 (x::l).
-Proof using. split; unfold length; rew_list~. Qed.
-
-Lemma ZInbound_zero_not_nil : forall x l,
-  l <> nil -> ZInbound 0 l.
-Proof using.
-  intros. split~. unfold length.
-  destruct l; tryfalse. rew_list~.
-Qed.
-
-Lemma ZInbound_cons : forall i j x l,
-  ZInbound j l -> j = i-1 -> ZInbound i (x::l).
-Proof using. introv [P U] H. split; rew_list~. Qed.
-
-Lemma ZInbound_nil_inv : forall i,
-  ZInbound i nil -> False.
-Proof using. introv [P U]. rew_list in U. math. Qed.
-
-Lemma ZInbound_cons_inv : forall i x l,
-  ZInbound i (x::l) -> i = 0 \/ (i <> 0 /\ ZInbound (i-1) l).
-Proof using.
-  introv [P U]. rew_length in U. tests: (i = 0).
-    left~.
-    right~. split. math. split~.
-Qed.
-
-Lemma ZInbound_cons_pos_inv : forall i x l,
-  ZInbound i (x::l) -> i <> 0 -> ZInbound (i-1) l.
-Proof using.
-  introv H P. destruct* (ZInbound_cons_inv H).
-Qed.
-
-Lemma ZInbound_one_pos_inv : forall i x,
-  ZInbound i (x::nil) -> i <> 0 -> False.
-Proof using.
-  intros. eapply ZInbound_nil_inv. apply* ZInbound_cons_pos_inv.
-Qed.
-
-Lemma ZInbound_app_l_inv : forall i l1 l2,
-  ZInbound i (l1++l2) -> i < length l1 -> ZInbound i l1.
-Proof using. introv [P U] H. split~. Qed.
-
-Lemma ZInbound_app_r_inv : forall i j l1 l2,
-  ZInbound j (l1++l2) -> j = length l1 + i -> i >= 0 -> ZInbound i l2.
-Proof using. introv [P U] R H. rew_length in U. split~. Qed.
-
-
-(* ---------------------------------------------------------------------- *)
-(** * DEPRECATED -- ZUpdate *)
-
-Lemma ZUpdate_here : forall x y l,
-  ZUpdate 0 x (y::l) (x::l).
-Proof using. split~. apply Update_here. Qed.
-
-Lemma ZUpdate_cons : forall i j x y l l',
-  ZUpdate j x l l' -> i = j+1 -> ZUpdate i x (y::l) (y::l').
-Proof using.
-  introv [U P] H. split~. applys_eq~ Update_cons 4.
-  subst. rew_abs_pos~.
-Qed.
-
-Lemma ZUpdate_app_l : forall i x l1 l1' l2,
-  ZUpdate i x l1 l1' -> ZUpdate i x (l1++l2) (l1'++l2).
-Proof using. introv [U P]. split~. apply~ Update_app_l. Qed.
-
-Lemma ZUpdate_app_r : forall i j x l1 l2 l2',
-  ZUpdate j x l2 l2' -> i = j + length l1 -> ZUpdate i x (l1++l2) (l1++l2').
-Proof using.
-  introv [U P] H. unfolds length. split~. apply~ Update_app_r.
-  subst. rew_abs_pos~.
-Qed.
-
-Lemma ZUpdate_not_nil : forall i x l1 l2,
-  ZUpdate i x l1 l2 -> l2 <> nil.
-Proof using. introv [U P]. apply~ Update_not_nil. Qed.
-
-Lemma ZUpdate_length : forall i x l l',
-  ZUpdate i x l l' -> length l = length l'.
-Proof using.
-  introv [U P]. unfolds length.
-  forwards~: Update_length.
-Qed.
-
-
-End ZindicesOld.
-
-(* -------------------------------------------------------------------------- *)
-
-(* The [prefix] ordering on lists has been defined in [LibList]. Here, we
-   provide an alternate definition, as well as more properties. *)
-
-(* TEMPORARY characterize [prefix] as pointwise equality *)
-
-Section Prefix.
-
-Variables (A : Type).
-Implicit Types xs ys : list A.
-
-Lemma le_implies_ge: forall x y, x <= y -> y >= x.
-Proof using. math. Qed.
-
-Local Hint Resolve le_implies_ge length_nonneg.
-
-(* [prefix], [snoc], and read access. *)
-
-Lemma prefix_read:
-  forall `{Inhab A} ys xs y,
-  prefix (ys & y) xs ->
-  y = xs[length ys].
-Proof using.
-  intros.
-  change (xs[length ys]) with (nth (length ys) xs).
-  unfold nth. case_if as Hop; [ | clear Hop ].
-  { false. forwards: length_nonneg ys. math. }
-  unfold LibList.nth.
-  generalize dependent xs.
-  generalize dependent ys. unfold prefix.
-  induction ys; intros xs [ zs ? ]; rew_list in *.
-  (* Base case. *)
-  { change (abs 0) with (0%nat).
-    subst xs. reflexivity. }
-  (* Inductive case. *)
-  { rewrite abs_plus by first [ math | eauto ].
-    change (abs 1) with (1%nat).
-    destruct xs as [ | x xs ]; [ congruence | ].
-    simpl. eapply IHys. exists zs. rew_list. congruence. }
-Qed.
-
-(* [prefix] and [length]. *)
-
-Lemma prefix_length:
-  forall ys xs,
-  prefix ys xs ->
-  length ys <= length xs.
-Proof using.
-  intros ys xs [ zs ? ]. subst xs. rew_list.
-  assert (length zs >= 0). { eauto. }
-  math.
-Qed.
-
-Lemma prefix_snoc_length:
-  forall ys y xs,
-  prefix (ys & y) xs ->
-  length ys < length xs.
-Proof using.
-  intros ys y xs [ zs ? ]. subst xs. rew_list.
-  assert (length zs >= 0). { eauto. }
-  math.
-Qed.
-
-End Prefix.
-
-
-
-(* -------------------------------------------------------------------------- *)
-(* TODO: cleanup *)
-
-Module TakeInt. (* TODO: move to LibListZ *)
-Import LibInt.
-Section Facts.
-Variables (A:Type).
-Implicit Types x : A.
-Implicit Types l : list A.
-
-Lemma take_cons_pred_int : forall x l (n:int),
-  n > 0 ->
-  take (abs n) (x::l) = x :: (take (abs (n-1)) l).
-Proof using. (* using stdlib *)
-  introv Pos. rewrite take_cons_pred.
-  rewrite abs_minus; try math. auto.
-  forwards: lt_abs_abs 0 n; math.
-Qed.
-
-Lemma take_cons_int : forall x l (n:int),
-  n >= 0 ->
-  take (abs (n+1)) (x::l) = x :: (take (abs n) l).
-Proof using.
-  introv Pos. rewrite~ abs_plus.
-  rewrite~ plus_comm. math.
-Qed.
-
-End Facts.
-End TakeInt.
-Export TakeInt.
+Ltac auto_tilde ::= auto_tilde_default.
